Dafny/examples/Challenge6/Challenge6Code.s.dfy
@@ -15,61 +15,7 @@ module challenge6Code{
     import opened memory
 
 
-    function challenge_prob_5_code_write_encrypted_simple():codeRe
-    {
-
-       // [temp] dummy ptrs
-        // var call := D(Ptr(0,0,0,1));
-        var call := LV("call");
-
-        var mblock := D(Ptr(0,0,0,1));
-        var call1 := LV("call1");
-        // var call2 := D(Ptr(0,0,0,1));
-        var call2 := LV("call2");//D(Int(0,IntType(1,false)));
-        var call3 := LV("call3");//D(Int(1,IntType(4,false)));
-
-        // var call3 := D(Ptr(0,0,0,1));
-        var call4 := D(Ptr(0,0,0,1));
-        var IV_SIZE := D(Int(16,IntType(4,false)));
-        var KEY := D(Int(16,IntType(4,false)));
-        var cipherText := D(Ptr(0,0,0,1));
-        var bytes_written := D(Ptr(0,0,0,1));
-
-        var cmp := LV("cmp");//D(Int(0,IntType(1,false)));
-        var cmp5 := D(Int(0,IntType(1,false)));
- 
-        var var_1 := D(Ptr(0,0,0,1));
-        var var_2 := D(Int(0,IntType(4,false)));
-        var var_3 := D(Ptr(0,0,0,1));
-    
-        var conv := D(Int(0,IntType(8,false)));
-
-
-    //   %bytes_written = alloca i32, align 4
-    //   call void @llvm.lifetime.start.p0i8(i64 4, i8* nonnull %0) #24
-    //   %call = tail call noalias align 16 dereferenceable_or_null(112) i8* @malloc(i64 112) #24
-    //   tail call void @llvm.memcpy.p0i8.p0i8.i64(i8* noundef nonnull align 16 dereferenceable(112) %call, i8* noundef nonnull align 8 dereferenceable(112) getelementptr inbounds (%struct.MBlock, %struct.MBlock* @mblock, i64 0, i32 0, i64 0), i64 112, i1 false)
-    //   %call1 = tail call noalias align 16 dereferenceable_or_null(120) i8* @malloc(i64 120) #24
-    //   %call2 = tail call i32 @encrypt(i8* %call, i32 112, i8* getelementptr inbounds ([32 x i8], [32 x i8]* @KEY, i64 0, i64 0), i8* getelementptr inbounds ([16 x i8], [16 x i8]* @IV, i64 0, i64 0), i8* %call1) #24
-    //   store i32 %call2, i32* %bytes_written, align 4, !tbaa !3
-    //   %1 = load %struct._IO_FILE*, %struct._IO_FILE** @wfd, align 8, !tbaa !14
-    //   %call3 = call i64 @fwrite(i8* nonnull %0, i64 4, i64 1, %struct._IO_FILE* %1)
-    //   %cmp = icmp eq i64 %call3, 0
-    //   br i1 %cmp, label %if.then, label %if.end
-    
-    //main function block
-       Block([Ins(CALL(call,malloc(Int(0,IntType(8,false))))),
-              Ins(LLVM_MEMCPY(call,mblock,1,false)),
-              Ins(CALL(call1,malloc(Ptr(0,0,0,1)))),
-              Ins(CALL(call2,encrypt(call,4,KEY,IV_SIZE,cipherText))),
-              Ins(STORE(call2,bytes_written)),
-              Ins(CALL(call3,fwrite_empty(bytes_written,4,1,D(Ptr(0,0,0,1))))),
-              Ins(ICMP(cmp,eq,4,call3,D(Int(0,IntType(4,false))))),
-              Ins(CALL(D(Void),stateOutputDump(KEY.d,IV_SIZE.d)))])
-    }
-
-
-    function challenge_prob_5_code_write_encrypted_simple_side_effect():codeRe
+    function challenge_prob_6_code_write_encrypted_simple_vuln():codeRe
     {
 
        // [temp] dummy ptrs
@@ -103,6 +49,7 @@ module challenge6Code{
     //   %bytes_written = alloca i32, align 4
     //   call void @llvm.lifetime.start.p0i8(i64 4, i8* nonnull %0) #24
     //   %call = tail call noalias align 16 dereferenceable_or_null(112) i8* @malloc(i64 112) #24
+    //   call void @crc32(i8* %call, i64 %conv, i8* %1)
     //   tail call void @llvm.memcpy.p0i8.p0i8.i64(i8* noundef nonnull align 16 dereferenceable(112) %call, i8* noundef nonnull align 8 dereferenceable(112) getelementptr inbounds (%struct.MBlock, %struct.MBlock* @mblock, i64 0, i32 0, i64 0), i64 112, i1 false)
     //   %call1 = tail call noalias align 16 dereferenceable_or_null(120) i8* @malloc(i64 120) #24
     //   %call2 = tail call i32 @encrypt(i8* %call, i32 112, i8* getelementptr inbounds ([32 x i8], [32 x i8]* @KEY, i64 0, i64 0), i8* getelementptr inbounds ([16 x i8], [16 x i8]* @IV, i64 0, i64 0), i8* %call1) #24
@@ -114,24 +61,166 @@ module challenge6Code{
     
     //main function block
        Block([Ins(CALL(call,malloc(Int(0,IntType(8,false))))),
+              Ins(CALL(D(Void),crc32(INTEGRITY_SIZE,mblock))),
               Ins(LLVM_MEMCPY(call,mblock,1,false)),
               Ins(CALL(call1,malloc(Ptr(0,0,0,1)))),
-              Ins(CALL(call2,encrypt_side_effects(INTEGRITY_SIZE))),
+              Ins(CALL(call2,encrypt(call,4,KEY,IV_SIZE,cipherText))),
               Ins(STORE(call2,bytes_written)),
               Ins(CALL(call3,fwrite_empty(bytes_written,4,1,D(Ptr(0,0,0,1))))),
               Ins(ICMP(cmp,eq,4,call3,D(Int(0,IntType(4,false))))),
-              Ins(CALL(D(Void),stateOutputDump(KEY.d,IV_SIZE.d)))])
+              Ins(CALL(D(Void),stateOutputDump(KEY,INTEGRITY_SIZE)))])
     }
 
-    function stateOutputDump(KEY:Data,IV_SIZE:Data):codeSeq
+    function challenge_prob_6_code_write_encrypted_simple_patch():codeRe
     {
-        [Ins(RET(D(KEY))),
-         Ins(RET(D(IV_SIZE)))]
+
+       // [temp] dummy ptrs
+        // var call := D(Ptr(0,0,0,1));
+        var call := LV("call");
+
+        var mblock := LV("mblock");
+        var call1 := LV("call1");
+        // var call2 := D(Ptr(0,0,0,1));
+        var call2 := LV("call2");//D(Int(0,IntType(1,false)));
+        var call3 := LV("call3");//D(Int(1,IntType(4,false)));
+        var INTEGRITY_SIZE := LV("INTEGRITY_SIZE");
+        var digestLength :=  LV("digestLength");
+        // var call3 := D(Ptr(0,0,0,1));
+        var call4 := D(Ptr(0,0,0,1));
+        var IV_SIZE := D(Int(16,IntType(4,false)));
+        var KEY := D(Int(16,IntType(4,false)));
+        var cipherText := D(Ptr(0,0,0,1));
+        var bytes_written := D(Ptr(0,0,0,1));
+
+        var cmp := LV("cmp");//D(Int(0,IntType(1,false)));
+        var cmp5 := D(Int(0,IntType(1,false)));
+ 
+        var var_1 := D(Ptr(0,0,0,1));
+        var var_2 := D(Int(0,IntType(4,false)));
+        var var_3 := D(Ptr(0,0,0,1));
+    
+        var conv := D(Int(0,IntType(8,false)));
+
+
+    //   %bytes_written = alloca i32, align 4
+    //   call void @llvm.lifetime.start.p0i8(i64 4, i8* nonnull %0) #24
+    //   %call = tail call noalias align 16 dereferenceable_or_null(112) i8* @malloc(i64 112) #24
+    //   call void @crc32(i8* %call, i64 %conv, i8* %1)
+    //   tail call void @llvm.memcpy.p0i8.p0i8.i64(i8* noundef nonnull align 16 dereferenceable(112) %call, i8* noundef nonnull align 8 dereferenceable(112) getelementptr inbounds (%struct.MBlock, %struct.MBlock* @mblock, i64 0, i32 0, i64 0), i64 112, i1 false)
+    //   %call1 = tail call noalias align 16 dereferenceable_or_null(120) i8* @malloc(i64 120) #24
+    //   %call2 = tail call i32 @encrypt(i8* %call, i32 112, i8* getelementptr inbounds ([32 x i8], [32 x i8]* @KEY, i64 0, i64 0), i8* getelementptr inbounds ([16 x i8], [16 x i8]* @IV, i64 0, i64 0), i8* %call1) #24
+    //   store i32 %call2, i32* %bytes_written, align 4, !tbaa !3
+    //   %1 = load %struct._IO_FILE*, %struct._IO_FILE** @wfd, align 8, !tbaa !14
+    //   %call3 = call i64 @fwrite(i8* nonnull %0, i64 4, i64 1, %struct._IO_FILE* %1)
+    //   %cmp = icmp eq i64 %call3, 0
+    //   br i1 %cmp, label %if.then, label %if.end
+    
+    //main function block
+       Block([Ins(CALL(call,malloc(Int(0,IntType(8,false))))),
+              Ins(CALL(D(Void),digest(digestLength,INTEGRITY_SIZE,mblock))),
+              Ins(LLVM_MEMCPY(call,mblock,1,false)),
+              Ins(CALL(call1,malloc(Ptr(0,0,0,1)))),
+              Ins(CALL(call2,encrypt(call,4,KEY,IV_SIZE,cipherText))),
+              Ins(STORE(call2,bytes_written)),
+              Ins(CALL(call3,fwrite_empty(bytes_written,4,1,D(Ptr(0,0,0,1))))),
+              Ins(ICMP(cmp,eq,4,call3,D(Int(0,IntType(4,false))))),
+              Ins(CALL(D(Void),stateOutputDump(KEY,INTEGRITY_SIZE)))])
+    }
+
+
+    function challenge_prob_6_code_write_encrypted_simple_patch_side_effect():codeRe
+    {
+
+       // [temp] dummy ptrs
+        // var call := D(Ptr(0,0,0,1));
+        var call := LV("call");
+
+        var mblock := D(Ptr(0,0,0,1));
+        var call1 := LV("call1");
+        // var call2 := D(Ptr(0,0,0,1));
+        var call2 := LV("call2");//D(Int(0,IntType(1,false)));
+        var call3 := LV("call3");//D(Int(1,IntType(4,false)));
+        var INTEGRITY_SIZE := LV("INTEGRITY_SIZE");
+        var digestLength :=  LV("digestLength");
+
+        // var call3 := D(Ptr(0,0,0,1));
+        var call4 := D(Ptr(0,0,0,1));
+        var IV_SIZE := D(Int(16,IntType(4,false)));
+        var KEY := D(Int(16,IntType(4,false)));
+        var cipherText := D(Ptr(0,0,0,1));
+        var bytes_written := D(Ptr(0,0,0,1));
+
+        var cmp := LV("cmp");//D(Int(0,IntType(1,false)));
+        var cmp5 := D(Int(0,IntType(1,false)));
+ 
+        var var_1 := D(Ptr(0,0,0,1));
+        var var_2 := D(Int(0,IntType(4,false)));
+        var var_3 := D(Ptr(0,0,0,1));
+    
+        var conv := D(Int(0,IntType(8,false)));
+
+
+    //   %bytes_written = alloca i32, align 4
+    //   call void @llvm.lifetime.start.p0i8(i64 4, i8* nonnull %0) #24
+    //   %call = tail call noalias align 16 dereferenceable_or_null(112) i8* @malloc(i64 112) #24
+    //   tail call void @llvm.memcpy.p0i8.p0i8.i64(i8* noundef nonnull align 16 dereferenceable(112) %call, i8* noundef nonnull align 8 dereferenceable(112) getelementptr inbounds (%struct.MBlock, %struct.MBlock* @mblock, i64 0, i32 0, i64 0), i64 112, i1 false)
+    //   %call1 = tail call noalias align 16 dereferenceable_or_null(120) i8* @malloc(i64 120) #24
+    //   %call2 = tail call i32 @encrypt(i8* %call, i32 112, i8* getelementptr inbounds ([32 x i8], [32 x i8]* @KEY, i64 0, i64 0), i8* getelementptr inbounds ([16 x i8], [16 x i8]* @IV, i64 0, i64 0), i8* %call1) #24
+    //   store i32 %call2, i32* %bytes_written, align 4, !tbaa !3
+    //   %1 = load %struct._IO_FILE*, %struct._IO_FILE** @wfd, align 8, !tbaa !14
+    //   %call3 = call i64 @fwrite(i8* nonnull %0, i64 4, i64 1, %struct._IO_FILE* %1)
+    //   %cmp = icmp eq i64 %call3, 0
+    //   br i1 %cmp, label %if.then, label %if.end
+    
+    //main function block
+        Block([Ins(CALL(call,malloc(Int(0,IntType(8,false))))),
+            Ins(CALL(digestLength,digest_side_effects(digestLength,INTEGRITY_SIZE,mblock))),
+            Ins(LLVM_MEMCPY(call,mblock,1,false)),
+            Ins(CALL(call1,malloc(Ptr(0,0,0,1)))),
+            Ins(CALL(call2,encrypt(call,4,KEY,IV_SIZE,cipherText))),
+            Ins(STORE(call2,bytes_written)),
+            Ins(CALL(call3,fwrite_empty(bytes_written,4,1,D(Ptr(0,0,0,1))))),
+            Ins(ICMP(cmp,eq,4,call3,D(Int(0,IntType(4,false))))),
+            Ins(CALL(D(Void),stateOutputDump(KEY,INTEGRITY_SIZE)))])
+
+    //    Block([Ins(CALL(call,malloc(Int(0,IntType(8,false))))),
+    //           Ins(LLVM_MEMCPY(call,mblock,1,false)),
+    //           Ins(CALL(call1,malloc(Ptr(0,0,0,1)))),
+    //           Ins(CALL(call2,encrypt_side_effects(INTEGRITY_SIZE))),
+    //           Ins(STORE(call2,bytes_written)),
+    //           Ins(CALL(call3,fwrite_empty(bytes_written,4,1,D(Ptr(0,0,0,1))))),
+    //           Ins(ICMP(cmp,eq,4,call3,D(Int(0,IntType(4,false))))),
+    //           Ins(CALL(D(Void),stateOutputDump(INTEGRITY_SIZE,IV_SIZE)))])
+    }
+
+    function stateOutputDump(KEY:operand,IV_SIZE:operand):codeSeq
+    {
+        [Ins(RET(KEY)),
+         Ins(RET(IV_SIZE))]
     }
  
     function encrypt(plainText:operand,size:nat,KEY:operand,IV:operand,cipherText:operand):codeSeq
     {
         [CNil]
+    }
+
+     
+    function crc32(INTEGRITY_SIZE:operand,mblock:operand):codeSeq //stub
+    {
+        [CNil]
+    }
+
+    function digest(digest:operand,INTEGRITY_SIZE:operand,mblock:operand):codeSeq //stub
+    {
+        [CNil]
+        // [Ins(ADD(digest,1,INTEGRITY_SIZE,digest))] + [CNil]
+    }
+
+
+    function digest_side_effects(digestLength:operand,INTEGRITY_SIZE:operand,mblock:operand):codeSeq
+    {
+
+        [Ins(SUB(INTEGRITY_SIZE,1,INTEGRITY_SIZE,D(Int(1,IntType(1,false)))))] + [CNil]
     }
 
     function encrypt_side_effects(INTEGRITY_SIZE:operand):codeSeq
@@ -181,7 +270,7 @@ module challenge6Code{
 
 ///////////////////////////////////////
 
-    predicate validInput(s:state, input:operand)
+    predicate validInput(s:state)
         requires ValidState(s)
     {
         && s.o.Nil?
@@ -200,30 +289,37 @@ module challenge6Code{
         var bytes_written := LV("bytes_written");
         var cmp := LV("cmp");
         var INTEGRITY_SIZE := LV("INTEGRITY_SIZE");
+        var digestLength := LV("digestLength");
         && ValidOperand(s,call)
         && ValidOperand(s,call1)
         && ValidOperand(s,call2)
         && ValidOperand(s,call3)
+        && ValidOperand(s,call4)
         && ValidOperand(s,mblock)
         && ValidOperand(s,cmp)
         && ValidOperand(s,bytes_written)
         && ValidOperand(s,INTEGRITY_SIZE)
+        && ValidOperand(s,digestLength)
         && s.lvs["call"].Ptr?
         && s.lvs["call1"].Ptr?
         && s.lvs["call2"].Int?
         && s.lvs["call3"].Int?
+        && s.lvs["call4"].Int?
         && s.lvs["mblock"].Ptr?
         && s.lvs["bytes_written"].Ptr?
         && s.lvs["cmp"].Int?
         && s.lvs["INTEGRITY_SIZE"].Int?
+        && s.lvs["digestLength"].Int?
         && s.lvs["call"] == (Ptr(0,0,0,1))
         && s.lvs["call1"] == (Ptr(0,0,0,1))
         && s.lvs["call2"] == (Int(0,IntType(1,false)))
         && s.lvs["mblock"] == (Ptr(0,0,0,1))
         && s.lvs["bytes_written"] == (Ptr(0,0,0,1))
         && s.lvs["call3"] == (Int(1,IntType(4,false)))
+        && s.lvs["call4"] == (Int(1,IntType(4,false)))
         && s.lvs["cmp"] == Int(0,IntType(1,false))
         && s.lvs["INTEGRITY_SIZE"] == Int(4,IntType(1,false))
+        && s.lvs["digestLength"] == Int(0,IntType(1,false))
         && s.m.mem[0][0].mb? 
         && s.m.mem[0][0].size == 1
         // && operandsUnique(s,[call,call1,call2,call3,mblock,bytes_written,cmp,INTEGRITY_SIZE])
