Dafny/examples/Challenge6/Challenge6CodeLemmasPatchSideEffect.i.dfy
@@ -5,8 +5,9 @@ include "../../LLVM/behaviorLemmas.i.dfy"
 include "../../Libraries/Seqs.s.dfy"
 include "../../LLVM/memory.i.dfy"
 include "Challenge6Code.s.dfy"
+include "../../LLVM/Operations/binaryOperations.i.dfy"
 
-module challenge6CodeLemmas{
+module challenge6CodeLemmasPatchSideEffect{
     import opened control_flow
     import opened LLVM_defRE
     import opened types
@@ -14,21 +15,21 @@ module challenge6CodeLemmas{
     import opened behavior_lemmas
     import opened memory
     import opened challenge6Code
-
+    import opened binary_operations_i
 
 // -- hechenxi@umich : chenxi
 
-lemma unwrapVulnBehaviors(s:state, input:operand, c:codeRe) returns (preB:behavior)
+lemma unwrapPatchSideEffectBehaviors(s:state, c:codeRe) returns (preB:behavior)
         requires ValidState(s);
         requires validStartingState(s);
-        requires c == challenge_prob_5_code_write_encrypted_simple();
+        requires c == challenge_prob_6_code_write_encrypted_simple_patch_side_effect();
 
         // -- input is valid -- ie. valid 16 bit integer 
-        requires validInput(s,input);
+        requires validInput(s);
         
         // ensures ValidBehaviorNonTrivial(preB);
-        ensures BehaviorEvalsCode(challenge_prob_5_code_write_encrypted_simple(),preB);
-        ensures |preB| == 10;
+        ensures BehaviorEvalsCode(challenge_prob_6_code_write_encrypted_simple_patch_side_effect(),preB);
+        ensures |preB| == 11;
         ensures preB[0] == s;
         
         ensures StateNext(preB[0],preB[1]);
@@ -56,7 +57,7 @@ lemma unwrapVulnBehaviors(s:state, input:operand, c:codeRe) returns (preB:behavi
         ensures ValidState(preB[9]);
         // ensures preB == [s] + evalCodeRE(c,s);
         // ensures 
-        ensures behaviorOutput(preB) == [Nil,
+       ensures behaviorOutput(preB) == [Nil,
                                         Nil,
                                         Nil,
                                         Nil,
@@ -64,9 +65,10 @@ lemma unwrapVulnBehaviors(s:state, input:operand, c:codeRe) returns (preB:behavi
                                         Nil,
                                         Nil,
                                         Nil,
-                                        SubOut([Out(Int(16,IntType(4,false))),Out(Int(16,IntType(4,false))),Out(Int(16,IntType(4,false)))]),
-                                        SubOut([Out(Int(16,IntType(4,false))),Out(Int(16,IntType(4,false))),Out(Int(16,IntType(4,false)))])];
-
+                                        Nil,
+                                        SubOut([Out((Int(16,IntType(4,false)))),Out(Int(3,IntType(1,false))),Out(Int(3,IntType(1,false)))]),
+                                        SubOut([Out((Int(16,IntType(4,false)))),Out(Int(3,IntType(1,false))),Out(Int(3,IntType(1,false)))])];
+    
 
 
     {
@@ -78,22 +80,24 @@ lemma unwrapVulnBehaviors(s:state, input:operand, c:codeRe) returns (preB:behavi
         var mblock:operand := LV("mblock");
         var call2 :=LV("call2");
         var call3 := LV("call3");
+        var call4 := LV("call4");
         assert OperandContents(s,call3).itype.size == 4;
+        var INTEGRITY_SIZE := LV("INTEGRITY_SIZE");
+        var digestLength :=  LV("digestLength");
 
         var cmp := LV("cmp");
-        var INTEGRITY_SIZE := LV("INTEGRITY_SIZE");
-
         var IV_SIZE := D(Int(16,IntType(4,false)));
         var KEY := D(Int(16,IntType(4,false)));
         var cipherText := D(Ptr(0,0,0,1));
         var bytes_written := D(Ptr(0,0,0,1));
 
         // var c := challenge_prob_5_code_write_encrypted_simple();
-        assert |c.block| == 8;
+         assert |c.block| == 9;
         preB := [s] + evalCodeRE(c,s);
        
         var step,remainder,subBehavior := unwrapBlockWitness(preB,c.block,s);
 
+            step,remainder,subBehavior := unwrapBlockWitness(subBehavior,remainder,last(step));
             step,remainder,subBehavior := unwrapBlockWitness(subBehavior,remainder,last(step));
             step,remainder,subBehavior := unwrapBlockWitness(subBehavior,remainder,last(step));
             step,remainder,subBehavior := unwrapBlockWitness(subBehavior,remainder,last(step));
@@ -107,72 +111,77 @@ lemma unwrapVulnBehaviors(s:state, input:operand, c:codeRe) returns (preB:behavi
         assert preB[1] == evalInsRe(CALL(call,malloc(Int(0,IntType(8,false)))),s);
         assert ValidOperand(preB[1],call);
 
-        assert NextStep(preB[1],preB[2],Step.evalInsStep(LLVM_MEMCPY(call,mblock,1,false)));
+        assert preB[2] == evalInsRe(CALL(digestLength,digest_side_effects(digestLength,INTEGRITY_SIZE,mblock)),preB[1]);
+        assert ValidInstruction(preB[1],CALL(digestLength,digest_side_effects(digestLength,INTEGRITY_SIZE,mblock)));
+        var sha := unwrapDigestSideEffectsWitness(preB[1],digestLength,digestLength,INTEGRITY_SIZE,mblock,preB[2]);
+        assert NextStep(preB[1],preB[2],Step.evalInsStep(CALL(digestLength,digest_side_effects(digestLength,INTEGRITY_SIZE,mblock))));
         assert StateNext(preB[1],preB[2]);
         assert ValidState(preB[2]);
-        assert preB[2] == evalInsRe(LLVM_MEMCPY(call,mblock,1,false),preB[1]);
-// 
-        assert preB[2] == preB[3];
-        assert NextStep(preB[2],preB[3],Step.evalInsStep(CALL(call1,malloc(Ptr(0,0,0,1)))));
-        assert ValidState(preB[3]);
+        // assert preB[2].o == SubOut([Nil]);
 
-        assert NextStep(preB[3],preB[4],Step.evalInsStep(CALL(call2,encrypt(call,4,KEY,IV_SIZE,cipherText))));
-        assert preB[3] == preB[4];
+        assert preB[2].o == Nil;
+        assert OperandContents(preB[2],INTEGRITY_SIZE).val == 3;
+
+        assert NextStep(preB[2],preB[3],Step.evalInsStep(LLVM_MEMCPY(call,mblock,1,false)));
+        assert StateNext(preB[2],preB[3]);
+        assert ValidState(preB[3]);
+        assert preB[3] == evalInsRe(LLVM_MEMCPY(call,mblock,1,false),preB[2]);
+
+         assert NextStep(preB[3],preB[4],Step.evalInsStep(CALL(call1,malloc(Ptr(0,0,0,1)))));
         assert ValidState(preB[4]);
-        
-        assert NextStep(preB[4],preB[5],Step.evalInsStep(STORE(call2,bytes_written)));
+
+        assert NextStep(preB[4],preB[5],Step.evalInsStep(CALL(call2,encrypt(call,4,KEY,IV_SIZE,cipherText))));
+        assert preB[4] == preB[5];
         assert ValidState(preB[5]);
         
-
-        assert ValidInstruction(preB[5],CALL(call3,fwrite(bytes_written,4,1,D(Ptr(0,0,0,1)))));
-        assert preB[6] == evalInsRe(CALL(call3,fwrite_empty(bytes_written,4,1,D(Ptr(0,0,0,1)))),preB[5]);
-        assert preB[5] == preB[6];
+        assert NextStep(preB[5],preB[6],Step.evalInsStep(STORE(call2,bytes_written)));
         assert ValidState(preB[6]);
+        
 
-        assert StateNext(preB[5],preB[6]);
-        assert ValidState(preB[6]);
+        assert ValidInstruction(preB[6],CALL(call3,fwrite(bytes_written,4,1,D(Ptr(0,0,0,1)))));
+        assert preB[6] == evalInsRe(CALL(call3,fwrite_empty(bytes_written,4,1,D(Ptr(0,0,0,1)))),preB[6]);
+        assert preB[6] == preB[7];
+        assert ValidState(preB[7]);
+        assert StateNext(preB[6],preB[7]);
+        assert ValidState(preB[7]);
         
         assert cmp.LV?;
         // var r := D(Int(0,IntType(4,false)));
         // assert  IntFits(r.d.val,r.d.itype);
-        var src2 := validZero16bitInt(preB[6]);
-        assert ValidOperand(preB[6],call3);// 
-        assert ValidOperand(preB[6],src2);
-        assert && isInt(OperandContents(preB[6],call3));// 
-        assert && isInt(OperandContents(preB[6],src2));
-        assert OperandContents(preB[6],call3).itype.size == 4;
-        assert !OperandContents(preB[6],call3).itype.signed;
-        intsTypeMatch(OperandContents(preB[6],call3),OperandContents(preB[6],src2));
-        assert typesMatch(OperandContents(preB[6],call3),OperandContents(preB[6],src2));
+        var src2 := validZero16bitInt(preB[7]);
+        assert ValidOperand(preB[7],call3);// 
+        assert ValidOperand(preB[7],src2);
+        assert && isInt(OperandContents(preB[7],call3));// 
+        assert && isInt(OperandContents(preB[7],src2));
+        assert OperandContents(preB[7],call3).itype.size == 4;
+        assert !OperandContents(preB[7],call3).itype.signed;
+        intsTypeMatch(OperandContents(preB[7],call3),OperandContents(preB[7],src2));
+        assert typesMatch(OperandContents(preB[7],call3),OperandContents(preB[7],src2));
 
-        // assert (Int(1,IntType(4,false))) == OperandContents(preB[6],call3);
-        assert ValidInstruction(preB[6],ICMP(cmp,eq,4,call3,src2));
+        // assert (Int(1,IntType(4,false))) == OperandContents(preB[7],call3);
+        assert ValidInstruction(preB[7],ICMP(cmp,eq,4,call3,src2));
 
-        assert preB[7] == evalInsRe(ICMP(cmp,eq,4,call3,src2),preB[6]);
-        // var s' := stateUpdateVar(preB[6],cmp,evalICMP(eq,4,OperandContents(preB[6],call3),OperandContents(preB[6],src2)));
+        assert preB[8] == evalInsRe(ICMP(cmp,eq,4,call3,src2),preB[7]);
+        // var s' := stateUpdateVar(preB[7],cmp,evalICMP(eq,4,OperandContents(preB[7],call3),OperandContents(preB[7],src2)));
 
 
-        assert NextStep(preB[6],preB[7],Step.evalInsStep(ICMP(cmp,eq,4,call3,src2)));
-        assert StateNext(preB[6],preB[7]);
-        assert ValidState(preB[7]);
+        assert NextStep(preB[7],preB[8],Step.evalInsStep(ICMP(cmp,eq,4,call3,src2)));
+        assert StateNext(preB[7],preB[8]);
+        assert ValidState(preB[8]);
 
-        assert ValidInstruction(preB[7],CALL(D(Void),stateOutputDump(KEY.d,IV_SIZE.d)));
+        assert ValidInstruction(preB[8],CALL(D(Void),stateOutputDump(KEY,INTEGRITY_SIZE)));
         // assert c[7] == CALL(D(Void),stateOutputDump(KEY,IV_SIZE));
-        assert preB[8] == evalInsRe(CALL(D(Void),stateOutputDump(KEY.d,IV_SIZE.d)),preB[7]);
-        var dump := unwrapDumpWitness(preB[7],KEY.d,IV_SIZE.d,preB[8]);
-        assert NextStep(preB[7],preB[8],Step.evalInsStep(CALL(D(Void),stateOutputDump(KEY.d,IV_SIZE.d))));   
-        assert preB[8].o == SubOut([Out((Int(16,IntType(4,false)))),Out(Int(16,IntType(4,false))),Out(Int(16,IntType(4,false)))]);
+        assert preB[9] == evalInsRe(CALL(D(Void),stateOutputDump(KEY,INTEGRITY_SIZE)),preB[8]);
+        var dump := unwrapDumpWitness(preB[8],KEY,INTEGRITY_SIZE,preB[9]);
+        assert NextStep(preB[8],preB[9],Step.evalInsStep(CALL(D(Void),stateOutputDump(KEY,INTEGRITY_SIZE))));   
+        assert preB[9].o == SubOut([Out((Int(16,IntType(4,false)))),Out(Int(3,IntType(1,false))),Out(Int(3,IntType(1,false)))]);
 
-        // // // LAST STEP
-        assert preB[8] == preB[9];
-        equalStatesAreStutter(preB[8],preB[9]);
+assert preB[9] == preB[10];
+        equalStatesAreStutter(preB[9],preB[10]);
         // assert ValidState(preB[8]);
         // assert NextStep(preB[7],preB[8],Step.stutterStep());
-        assert StateNext(preB[8],preB[9]);
+        assert StateNext(preB[9],preB[10]);
 
-        // // assert ValidBehaviorNonTrivial(preB);
-        // // assert BehaviorEvalsCode(c,preB);
-        assert |preB| == 10;
         assert behaviorOutput(preB) == [Nil,
                                         Nil,
                                         Nil,
@@ -181,34 +190,28 @@ lemma unwrapVulnBehaviors(s:state, input:operand, c:codeRe) returns (preB:behavi
                                         Nil,
                                         Nil,
                                         Nil,
-                                        SubOut([Out(Int(16,IntType(4,false))),Out(Int(16,IntType(4,false))),Out(Int(16,IntType(4,false)))]),
-                                        SubOut([Out(Int(16,IntType(4,false))),Out(Int(16,IntType(4,false))),Out(Int(16,IntType(4,false)))])];
-
-
+                                        Nil,
+                                        SubOut([Out((Int(16,IntType(4,false)))),Out(Int(3,IntType(1,false))),Out(Int(3,IntType(1,false)))]),
+                                        SubOut([Out((Int(16,IntType(4,false)))),Out(Int(3,IntType(1,false))),Out(Int(3,IntType(1,false)))])];
     }
 
-
-
- lemma vulnBehaviorIsValid(s:state, input:operand) returns (preB:behavior)
+ lemma PatchBehaviorIsValid(s:state) returns (preB:behavior)
         requires ValidState(s);
         requires validStartingState(s);
 
         // -- input is valid -- ie. valid 16 bit integer 
-        requires validInput(s,input);
+        requires validInput(s);
 
     {
         reveal_ValidBehavior();
         reveal_BehaviorEvalsCode();
-        var c := challenge_prob_5_code_write_encrypted_simple();
-        var x := unwrapVulnBehaviors(s,input,c);
+        var c := challenge_prob_6_code_write_encrypted_simple_patch_side_effect();
+        var x := unwrapPatchSideEffectBehaviors(s,c);
         assert ValidBehaviorNonTrivial(x);
         assert BehaviorEvalsCode(c,x);
 
-        // assert behaviorOutput(x) == [Nil,Nil,Nil,Nil,Nil,Nil,Out(x[5].lvs["bytes_written"]),Nil,Nil];
 
-        // assert BehaviorEvalsCode(c,preB);
     }
-
 
     lemma equalStatesAreStutter(s:state,s':state)
         requires s==s'
@@ -243,10 +246,134 @@ lemma unwrapVulnBehaviors(s:state, input:operand, c:codeRe) returns (preB:behavi
         val
     }
 
-    lemma unwrapDumpWitness(s:state,op1:Data,op2:Data,sNext:state) returns (b:behavior)
+lemma unwrapDigestSideEffectsWitness(s:state,dst:operand,digest:operand,INTEGRITY_SIZE:operand, mblock:operand,sNext:state) returns (b:behavior)
         requires ValidState(s)
-        requires ValidData(s,op1)
-        requires ValidData(s,op2)
+        requires ValidOperand(s,INTEGRITY_SIZE)
+        requires ValidOperand(s,dst)
+        requires dst != INTEGRITY_SIZE;
+        requires dst.LV?;
+        requires OperandContents(s,dst).Int?;
+        requires dst.l in s.lvs;
+        requires INTEGRITY_SIZE.LV?;
+        requires INTEGRITY_SIZE.l in s.lvs;
+        requires isInt(OperandContents(s,INTEGRITY_SIZE));
+        requires OperandContents(s,INTEGRITY_SIZE).itype.size == 1;
+        requires typesMatch(OperandContents(s,INTEGRITY_SIZE),OperandContents(s,D(Int(1,IntType(1,false)))))
+        requires OperandContents(s,INTEGRITY_SIZE).val == 4;
+        requires sNext == evalInsRe(CALL(dst,encrypt_side_effects(INTEGRITY_SIZE)),s);
+        requires ValidInstruction(s,CALL(dst,encrypt_side_effects(INTEGRITY_SIZE)));
+        requires s.o == Nil
+        ensures ValidBehavior(b);
+        ensures |b| == 3
+        ensures ValidOperand(last(b),dst)
+        ensures OperandContents(last(b),dst) == OperandContents(s,dst);
+
+        ensures ValidOperand(last(b),INTEGRITY_SIZE) && OperandContents(last(b),INTEGRITY_SIZE).Int?
+        ensures OperandContents(last(b),INTEGRITY_SIZE).val == 3;
+         ensures NextStep(s,sNext,Step.evalInsStep(CALL(dst,encrypt_side_effects(INTEGRITY_SIZE))));
+        ensures StateNext(s,sNext);
+        ensures ValidState(sNext);
+        ensures ValidOperand(sNext,INTEGRITY_SIZE);
+        // ensures OperandContents(s,dst) == OperandContents(last(b),dst);
+        ensures sNext == last(b).(o := Nil);
+        ensures behaviorOutput(b) == [Nil,Nil,Nil]
+        ensures OperandContents(sNext,INTEGRITY_SIZE) == Int(3,IntType(1,false));
+        ensures forall v :: (INTEGRITY_SIZE != v && ValidOperand(s,v)) ==> (ValidOperand(sNext,v) && OperandContents(sNext,v) == OperandContents(s,v));
+        ensures s.m == sNext.m;
+    {
+        reveal_behaviorOutput();
+        reveal_ValidBehavior();
+        var subB := [s] + evalCodeRE(Block(encrypt_side_effects(INTEGRITY_SIZE)),s);
+        assert encrypt_side_effects(INTEGRITY_SIZE) == [Ins(SUB(INTEGRITY_SIZE,1,INTEGRITY_SIZE,D(Int(1,IntType(1,false))))),CNil];
+        var step,remainder,subBehavior := unwrapBlockWitness(subB,encrypt_side_effects(INTEGRITY_SIZE),s);
+        step,remainder,subBehavior := unwrapBlockWitness(subBehavior,remainder,last(step));
+        // step,remainder,subBehavior := unwrapBlockWitness(subBehavior,remainder,last(step));
+         assert subB[0] == s;
+         assert subB[1] == evalInsRe(SUB(INTEGRITY_SIZE,1,INTEGRITY_SIZE,D(Int(1,IntType(1,false)))),s);
+         assert NextStep(subB[0],subB[1],Step.evalInsStep(SUB(INTEGRITY_SIZE,1,INTEGRITY_SIZE,D(Int(1,IntType(1,false))))));
+         assert subB[1] == subB[2];
+        assert subB[2] == stateUpdateVar(s,INTEGRITY_SIZE,evalSUB(1,OperandContents(s,INTEGRITY_SIZE),(Int(1,IntType(1,false)))));
+        // assert dst.l in subB[1].lvs;
+        // assert dst.l != INTEGRITY_SIZE.l;
+        assert forall lv :: (lv in s.lvs && lv != INTEGRITY_SIZE.l) ==> subB[1].lvs[lv] == s.lvs[lv];
+
+        // assert s.lvs[dst.l] == subB[1].lvs[dst.l];
+        //  assert OperandContents(s,dst) == OperandContents(subB[1],dst);
+         equalStatesAreStutter(subB[1],subB[2]);
+         assert StateNext(subB[1],subB[2]);
+         assert |subB| == 3;
+         assert subB[2] == last(subB);
+         assert  OperandContents(subB[2],INTEGRITY_SIZE).val == 3;
+         assert ValidBehavior(subB);
+         return subB;
+    }
+
+    lemma unwrapEncryptSideEffectsWitness(s:state,dst:operand,INTEGRITY_SIZE:operand, sNext:state) returns (b:behavior)
+        requires ValidState(s)
+        requires ValidOperand(s,INTEGRITY_SIZE)
+        requires ValidOperand(s,dst)
+        requires dst != INTEGRITY_SIZE;
+        requires dst.LV?;
+        requires OperandContents(s,dst).Int?;
+        requires dst.l in s.lvs;
+        requires INTEGRITY_SIZE.LV?;
+        requires INTEGRITY_SIZE.l in s.lvs;
+        requires isInt(OperandContents(s,INTEGRITY_SIZE));
+        requires OperandContents(s,INTEGRITY_SIZE).itype.size == 1;
+        requires typesMatch(OperandContents(s,INTEGRITY_SIZE),OperandContents(s,D(Int(1,IntType(1,false)))))
+        requires OperandContents(s,INTEGRITY_SIZE).val == 4;
+        requires sNext == evalInsRe(CALL(dst,encrypt_side_effects(INTEGRITY_SIZE)),s);
+        requires ValidInstruction(s,CALL(dst,encrypt_side_effects(INTEGRITY_SIZE)));
+        requires s.o == Nil
+        ensures ValidBehavior(b);
+        ensures |b| == 3
+        ensures ValidOperand(last(b),dst)
+        // ensures OperandContents(last(b),dst) == OperandContents(s,dst);
+
+        ensures ValidOperand(last(b),INTEGRITY_SIZE) && OperandContents(last(b),INTEGRITY_SIZE).Int?
+        ensures OperandContents(last(b),INTEGRITY_SIZE).val == 3;
+         ensures NextStep(s,sNext,Step.evalInsStep(CALL(dst,encrypt_side_effects(INTEGRITY_SIZE))));
+        ensures StateNext(s,sNext);
+        ensures ValidState(sNext);
+        ensures ValidOperand(sNext,INTEGRITY_SIZE);
+        // ensures OperandContents(s,dst) == OperandContents(last(b),dst);
+        ensures sNext == last(b).(o := Nil);
+        ensures behaviorOutput(b) == [Nil,Nil,Nil]
+        ensures OperandContents(sNext,INTEGRITY_SIZE) == Int(3,IntType(1,false));
+        ensures forall v :: (INTEGRITY_SIZE != v && ValidOperand(s,v)) ==> (ValidOperand(sNext,v) && OperandContents(sNext,v) == OperandContents(s,v));
+        ensures s.m == sNext.m;
+    {
+        reveal_behaviorOutput();
+        reveal_ValidBehavior();
+        var subB := [s] + evalCodeRE(Block(encrypt_side_effects(INTEGRITY_SIZE)),s);
+        assert encrypt_side_effects(INTEGRITY_SIZE) == [Ins(SUB(INTEGRITY_SIZE,1,INTEGRITY_SIZE,D(Int(1,IntType(1,false))))),CNil];
+        var step,remainder,subBehavior := unwrapBlockWitness(subB,encrypt_side_effects(INTEGRITY_SIZE),s);
+        step,remainder,subBehavior := unwrapBlockWitness(subBehavior,remainder,last(step));
+        // step,remainder,subBehavior := unwrapBlockWitness(subBehavior,remainder,last(step));
+         assert subB[0] == s;
+         assert subB[1] == evalInsRe(SUB(INTEGRITY_SIZE,1,INTEGRITY_SIZE,D(Int(1,IntType(1,false)))),s);
+         assert NextStep(subB[0],subB[1],Step.evalInsStep(SUB(INTEGRITY_SIZE,1,INTEGRITY_SIZE,D(Int(1,IntType(1,false))))));
+         assert subB[1] == subB[2];
+        assert subB[2] == stateUpdateVar(s,INTEGRITY_SIZE,evalSUB(1,OperandContents(s,INTEGRITY_SIZE),(Int(1,IntType(1,false)))));
+        assert dst.l in subB[1].lvs;
+        assert dst.l != INTEGRITY_SIZE.l;
+        assert forall lv :: (lv in s.lvs && lv != INTEGRITY_SIZE.l) ==> subB[1].lvs[lv] == s.lvs[lv];
+
+        assert s.lvs[dst.l] == subB[1].lvs[dst.l];
+        //  assert OperandContents(s,dst) == OperandContents(subB[1],dst);
+         equalStatesAreStutter(subB[1],subB[2]);
+         assert StateNext(subB[1],subB[2]);
+         assert |subB| == 3;
+         assert subB[2] == last(subB);
+         assert  OperandContents(subB[2],INTEGRITY_SIZE).val == 3;
+         assert ValidBehavior(subB);
+         return subB;
+    }
+
+    lemma unwrapDumpWitness(s:state,op1:operand,op2:operand,sNext:state) returns (b:behavior)
+        requires ValidState(s)
+        requires ValidOperand(s,op1)
+        requires ValidOperand(s,op2)
         requires sNext == evalInsRe(CALL(D(Void),stateOutputDump(op1,op2)),s)
         requires ValidInstruction(s,CALL(D(Void),stateOutputDump(op1,op2)));
         requires s.o == Nil
@@ -255,37 +382,37 @@ lemma unwrapVulnBehaviors(s:state, input:operand, c:codeRe) returns (preB:behavi
         ensures ValidBehavior(b);
         ensures ValidOperand(last(b),D(Void));
         // ensures ValidOperand(b[1],op2);
-        ensures behaviorOutput(b) == [Nil,Out(op1),Out(op2),Out(op2)];
+        ensures behaviorOutput(b) == [Nil,Out(OperandContents(s,op1)),Out(OperandContents(s,op2)),Out(OperandContents(s,op2))];
         ensures NextStep(s,sNext,Step.evalInsStep(CALL(D(Void),stateOutputDump(op1,op2))));
         ensures StateNext(s,sNext);
         ensures ValidState(sNext);
-        ensures sNext.o == SubOut([Out(op1),Out(op2),Out(op2)]);
+        ensures sNext.o == SubOut([Out(OperandContents(s,op1)),Out(OperandContents(s,op2)),Out(OperandContents(s,op2))]);
 
     {
         reveal_behaviorOutput();
         var subB := [s] + evalCodeRE(Block(stateOutputDump(op1,op2)),s);// alBlockRE(stateOutputDump(op1,op2),s);
-        assert stateOutputDump(op1,op2) == [Ins(RET(D(op1))),Ins(RET(D(op2)))];
+        assert stateOutputDump(op1,op2) == [Ins(RET((op1))),Ins(RET((op2)))];
 
         var step,remainder,subBehavior := unwrapBlockWitness(subB,stateOutputDump(op1,op2),s);
         step,remainder,subBehavior := unwrapBlockWitness(subBehavior,remainder,last(step));
         step,remainder,subBehavior := unwrapBlockWitness(subBehavior,remainder,last(step));
         
         assert subB[0] == s;
-        assert NextStep(subB[0],subB[1],Step.evalInsStep(RET(D(op1))));
+        assert NextStep(subB[0],subB[1],Step.evalInsStep(RET((op1))));
         assert ValidState(subB[1]);
-        assert subB[1].o == Out(op1);
-        assert NextStep(subB[1],subB[2],Step.evalInsStep(RET(D(op2))));
+        assert subB[1].o == Out(OperandContents(s,op1));
+        assert NextStep(subB[1],subB[2],Step.evalInsStep(RET((op2))));
         assert ValidState(subB[2]);
-        assert subB[2].o == Out(op2);
+        assert subB[2].o == Out(OperandContents(s,op2));
         assert subB[2] == subB[3];
         equalStatesAreStutter(subB[2],subB[3]);
         assert StateNext(subB[2],subB[3]);
-        assert behaviorOutput(subB) == [Nil,Out(op1),Out(op2),Out(op2)];
+        assert behaviorOutput(subB) == [Nil,Out(OperandContents(s,op1)),Out(OperandContents(s,op2)),Out(OperandContents(s,op2))];
         assert sNext == evalInsRe(CALL(D(Void),stateOutputDump(op1,op2)),s);
         assert sNext.ok;
         var rest := evalBlockRE(stateOutputDump(op1,op2),s);
         assert subB == [s] + rest;
-        assert behaviorOutput(rest) == [Out(op1),Out(op2),Out(op2)];
+        assert behaviorOutput(rest) == [Out(OperandContents(s,op1)),Out(OperandContents(s,op2)),Out(OperandContents(s,op2))];
         assert sNext.o == SubOut(behaviorOutput(rest));
         return subB;
     }
